Readme.lean
@@ -1,0 +1,22 @@
+import Spec
+import Std.Time.Time.Unit.Basic
+import Std.Time.Time.Unit.Second
+
+open Spec
+
+def oneSecondMs : Std.Time.Millisecond.Offset :=
+  Std.Time.Millisecond.Offset.ofSeconds (1 : Std.Time.Second.Offset)
+
+example : Spec := it "sometest" (do IO.println "ok")
+example : Spec := it (focus := true) "sometest" (do IO.println "ok")
+example : Spec := it (timeoutMs? := .some oneSecondMs) "sometest" (do IO.println "ok")
+example : Spec := it (focus := true) (timeoutMs? := .some oneSecondMs) "sometest" (do IO.println "ok")
+example : Spec := it (focus := true) "sometest" (timeoutMs? := .some oneSecondMs) (do IO.println "ok")
+example : Spec := it "sometest" (timeoutMs? := .some oneSecondMs) (focus := true) (do IO.println "ok")
+
+example : Spec := Spec.it "sometest" (do IO.println "ok")
+example : Spec := Spec.it (focus := true) "sometest" (do IO.println "ok")
+example : Spec := Spec.it (timeoutMs? := .some oneSecondMs) "sometest" (do IO.println "ok")
+example : Spec := Spec.it (focus := true) (timeoutMs? := .some oneSecondMs) "sometest" (do IO.println "ok")
+example : Spec := Spec.it (timeoutMs? := .some oneSecondMs) (focus := true) "sometest" (do IO.println "ok")
+example : Spec := Spec.it "sometest" (timeoutMs? := .some oneSecondMs) (focus := true) (do IO.println "ok")
